Simpler correctness/completeness.

LambdaS5/caml/jsParser.ml
@@ -6,9 +6,9 @@ let parsecmd = ref ""
 
 let set_parsecmd s = parsecmd := s
 
-let parse_file filename = 
-    try Some (Translate_syntax.coq_syntax_from_file filename)
-    with e -> None
+let parse_file filename =
+    try Some (Translate_syntax.coq_syntax_from_file ~force_strict:false filename)
+    with e -> Printexc.print_backtrace stdout; print_endline (Printexc.to_string e);None
 
 let parse s = 
     let filename = File.with_temporary_out (fun o fn -> String.print o s; fn) in
